started proving the generic theorem

src_arrays/Dijkstra_generic.v
@@ -10,6 +10,7 @@ Require Import src_arrays.LambdaTotalTriple_credits_perm.
 Require Import src_arrays.LamRefLogicFactsTotal_credits_perm.
 Require Import Lia.
 Require Import src_arrays.Tactics.
+Require Import src_arrays.SA_Tactics.
 Require Import src_arrays.Interweave.
 
 Require Import graphs.Graphs.
@@ -161,23 +162,24 @@ Definition get_size_spec {A} (get_size : Value A) : Prop :=
   forall vg g c,
     get_size_cost c ->
     triple_fun get_size
-      (fun v => <[v = vg]> <*> is_weighted_graph g vg)
+      (fun v => $c <*> <[v = vg]> <*> is_weighted_graph g vg)
       (fun v => <exists> n,
-        $ c <*> <[v = Int (Z.of_nat n)]> <*> <[is_set_size (V g) n]> <*>
-          is_weighted_graph g vg).
+        <[v = Int (Z.of_nat n)]> <*> <[is_set_size (V g) n]> <*>
+        is_weighted_graph g vg).
 
 Parameter get_neighbours_cost : forall (c : nat), Prop.
 
 Definition get_neighbours_spec {A} (get_neighbours : Value A) : Prop :=
   forall vg n (g : wgraph nat) c,
+    get_neighbours_cost c ->
     triple_fun get_neighbours
-      (fun v => <[v = vg]>)
+      (fun v => $1 <*> <[v = vg]>)
       (fun v => <[
         triple_fun v
-          (fun v => <[v = Int (Z.of_nat n)]> <*> <[V g n]> <*>
+          (fun v => $c <*> <[v = Int (Z.of_nat n)]> <*> <[V g n]> <*>
             is_weighted_graph g vg)
           (fun v => <exists> L,
-            $c <*> <[is_elem_weighted_unique_list (neighbours g n) (W g n) L]> <*>
+            <[is_elem_weighted_unique_list (neighbours g n) (W g n) L]> <*>
             is_list (nat_pairs2values L) v </\> is_weighted_graph g vg)
       ]>).
 
@@ -187,18 +189,24 @@ Definition get_max_label_spec {A} (get_max_label : Value A) : Prop :=
   forall vg g c,
     get_max_label_cost c ->
     triple_fun get_max_label
-      (fun v => <[v = vg]> <*> is_weighted_graph g vg)
+      (fun v => $c <*> <[v = vg]> <*> is_weighted_graph g vg)
       (fun v => <exists> C,
-        $c <*> <[v = Int (Z.of_nat C)]> <*> <[is_max_label g C]> <*>
-          is_weighted_graph g vg).
+        <[v = Int (Z.of_nat C)]> <*> <[is_max_label g C]> <*>
+        is_weighted_graph g vg).
 
 Parameter is_heap :
-  forall {V} (n C : nat) (P : nat -> Prop) (W : nat -> option nat),
+  forall {V} (n C : nat) (P : nat -> Prop) (W : nat -> option nat)
+    (* asymptotic number of credits required to extract all the elements *)
+    (potential : nat),
     Value V -> StateAssertion V.
 
+Parameter heap_time_bound :
+  forall (n C t : nat), Prop.
+
+(*
 Parameter place_in_heap :
   forall {V} (h : Value V) (x p : nat), Prop.
-
+*)
 
 Parameter mkheap_cost : forall (n C c : nat), Prop.
 
@@ -206,46 +214,49 @@ Definition mkheap_spec {V} (mkheap : Value V) : Prop :=
   forall n C c,
     mkheap_cost n C c ->
     triple_fun mkheap
-      (fun v => <[v = Int (Z.of_nat n)]>)
+      (fun v => $1 <*> <[v = Int (Z.of_nat n)]>)
       (fun v => <[
         triple_fun v
           (fun v => $c <*> <[v = Int (Z.of_nat C)]>)
-          (is_heap n C empty (fun _ => None))
+          (is_heap n C empty (fun _ => None) 0)
       ]>).
 
 Definition set_value_at (W : nat -> option nat) (x y n : nat) : option nat :=
   if n =? x then Some y else W n.
 
-Parameter h_insert_cost : forall (n C c : nat), Prop.
+(*Parameter h_insert_cost : forall (n C c : nat), Prop.*)
 
 Definition h_insert_spec {V} (h_insert : Value V) : Prop :=
-  forall n C (P : nat -> Prop) (W : nat -> option nat) h (s k d c : nat),
-    h_insert_cost n C c ->
+  forall n C (P : nat -> Prop) (W : nat -> option nat) h (p s k d c t : nat),
+    (*h_insert_cost n C c ->*)
+    c = t ->
+    heap_time_bound n C t ->
     is_set_size P s ->
     s < n ->
     ~ P k ->
     triple_fun h_insert
-      (fun v => <[v = h]>)
+      (fun v => $1 <*> <[v = h]>)
       (fun v => <[
         triple_fun v
-          (fun v => <[v = Int (Z.of_nat k)]>)
+          (fun v => $1 <*> <[v = Int (Z.of_nat k)]>)
           (fun v => <[
             triple_fun v
-              (fun v => $c <*> <[v = Int (Z.of_nat d)]> <*> is_heap n C P W h)
+              (fun v => $c <*> <[v = Int (Z.of_nat d)]> <*> is_heap n C P W p h)
               (fun v => (<exists> c', $c') <*> <[v = U_val]> <*>
-                is_heap n C (set_sum P (single k)) (set_value_at W k d) h)
+                <exists> p', <[p' < p + t]> <*>
+                  is_heap n C (set_sum P (single k)) (set_value_at W k d) p' h)
           ]>)
       ]>).
 
 Parameter h_empty_cost : forall (c : nat), Prop.
 
 Definition h_empty_spec {V} (h_empty : Value V) : Prop :=
-  forall n C (P : nat -> Prop) (W : nat -> option nat) h s c,
+  forall n C (P : nat -> Prop) (W : nat -> option nat) h s c p,
     h_empty_cost c ->
     is_set_size P s ->
     triple_fun h_empty
-      (fun v => <[v = h]> <*> is_heap n C P W h)
-      (fun v => <[v = Bool (s =? 0)]> <*> is_heap n C P W h).
+      (fun v => $1 <*> <[v = h]> <*> is_heap n C P W p h)
+      (fun v => <[v = Bool (s =? 0)]> <*> is_heap n C P W p h).
 
 Definition unset_value_at (W : nat -> option nat) (x n : nat) : option nat :=
   if n =? x then None else W n.
@@ -256,39 +267,41 @@ Definition set_remove {A} (P : A -> Prop) (x y : A) : Prop :=
 Parameter h_extract_min_cost : forall {V} (c : nat) (h : Value V), StateAssertion V.
 
 Definition h_extract_min_spec {V} (h_extract_min : Value V) : Prop :=
-  forall n C (P : nat -> Prop) (W : nat -> option nat) h k d c,
+  forall n C (P : nat -> Prop) (W : nat -> option nat) p h k d c,
     min_cost_elem P W k ->
     W k = Some d ->
     triple_fun h_extract_min
-      (fun v => $c <*> <[v = h]> <*> is_heap n C P W h </\> h_extract_min_cost c h)
-      (fun v => <[v = pair2Value nat2value nat2value (k,d)]> <*>
-        is_heap n C (set_remove P k) W h).
+      (fun v => $c <*> <[v = h]> <*> is_heap n C P W p h </\> h_extract_min_cost c h)
+      (fun v => (<exists> c', $c') <*> <[v = pair2Value nat2value nat2value (k,d)]> <*>
+        <exists> p', <[p = p' + c]> <*> is_heap n C (set_remove P k) W p' h).
 
 Parameter h_decrease_key_cost : forall {V} (c : nat) (h : Value V), StateAssertion V.
 
 Definition h_decrease_key_spec {V} (h_decrease_key : Value V) : Prop :=
-  forall n C (P : nat -> Prop) (W : nat -> option nat) h k d c,
+  forall n C (P : nat -> Prop) (W : nat -> option nat) p h k d c,
   P k ->
   triple_fun h_decrease_key
-    (fun v => <[v = h]>)
+    (fun v => $1 <*> <[v = h]>)
     (fun v => <[
       triple_fun v
-        (fun v => <[v = Int (Z.of_nat k)]>)
+        (fun v => $1 <*> <[v = Int (Z.of_nat k)]>)
         (fun v => <[
           triple_fun v
             (fun v => $c <*> <[v = Int (Z.of_nat d)]> <*>
-              is_heap n C P W h </\> h_decrease_key_cost c h)
-            (fun v => <[v = U_val]> <*> is_heap n C P (set_value_at W k d) h)
+              is_heap n C P W p h </\> h_decrease_key_cost c h)
+            (fun v => (<exists> c', $c') <*> <[v = U_val]> <*>
+              <exists> p', <[p = p' + c]> <*> is_heap n C P (set_value_at W k d) p' h)
         ]>)
     ]>).
 
-Parameter h_free_cost : forall (n C c : nat), Prop.
+Parameter h_free_cost : forall (n C s c : nat), Prop.
 
 Definition h_free_spec {V} (h_free : Value V) : Prop :=
-  forall n C (P : nat -> Prop) (W : nat -> option nat) c,
-  h_free_cost n C c ->
+  forall n C (P : nat -> Prop) (W : nat -> option nat) s c p,
+  is_set_size P s ->
+  h_free_cost n C s c ->
   triple_fun h_free
-    (is_heap n C P W <*>+ $c)
+    (is_heap n C P W p <*>+ $c)
     (fun v => <exists> c', $c').
 
 Definition is_nil_b {A} (L : list A) : bool :=
@@ -297,31 +310,51 @@ Definition is_nil_b {A} (L : list A) : bool :=
   | _ => false
   end.
 
+Parameter l_is_nil_cost : forall (c : nat), Prop.
+
 Definition l_is_nil_spec {V} (l_is_nil : Value V) : Prop :=
-  forall (L : list (Value V)) l,
+  forall (L : list (Value V)) l c,
+    l_is_nil_cost c ->
     triple_fun l_is_nil
-      (fun v => <[v = l]> <*> is_list L l)
+      (fun v => $c <*> <[v = l]> <*> is_list L l)
       (fun v => <[v = Bool (is_nil_b L)]> <*> is_list L l).
 
+Parameter l_head_cost : forall (c : nat), Prop.
+
 Definition l_head_spec {V} (l_head : Value V) : Prop :=
-  forall (L : list (Value V)) h l,
+  forall (L : list (Value V)) h l c,
+    l_head_cost c ->
     triple_fun l_head
-      (fun v => <[v = l]> <*> is_list (h::L)%list l)
+      (fun v => $ c <*> <[v = l]> <*> is_list (h::L)%list l)
       (fun v => <[v = h]> <*> is_list (h::L)%list l).
 
+Parameter l_tail_cost : forall (c : nat), Prop.
+
 Definition l_tail_spec {V} (l_tail : Value V) : Prop :=
-  forall (L : list (Value V)) h l t,
+  forall (L : list (Value V)) h l t c,
+    l_tail_cost c ->
     triple_fun l_tail
-      (fun v => <[v = l]> <*> is_list (h::L)%list l)
+      (fun v => $c <*> <[v = l]> <*> is_list (h::L)%list l)
       (fun v => <[v = t]> <*> is_list (h::L)%list l </\> is_list L t).
 
 Theorem triple_fun_generic_dijkstra
-  (get_size get_neighbours get_max_label mkheap h_insert h_empty
-    h_extract_min h_decrease_key h_free l_is_nil l_head l_tail : Value string)
-  (g : wgraph nat) l src D pred :
+  (get_size get_max_label get_neighbours mkheap h_insert h_empty
+    h_extract_min h_decrease_key h_free l_is_nil l_head l_tail : Value string) :
+  is_closed_value get_size ->
+  is_closed_value get_max_label ->
+  is_closed_value get_neighbours ->
+  is_closed_value mkheap ->
+  is_closed_value h_insert ->
+  is_closed_value h_empty ->
+  is_closed_value h_extract_min ->
+  is_closed_value h_decrease_key ->
+  is_closed_value h_free ->
+  is_closed_value l_is_nil ->
+  is_closed_value l_head ->
+  is_closed_value l_tail ->
   get_size_spec       get_size ->
-  get_neighbours_spec get_neighbours ->
   get_max_label_spec  get_max_label ->
+  get_neighbours_spec get_neighbours ->
   mkheap_spec         mkheap ->
   h_insert_spec       h_insert ->
   h_empty_spec        h_empty ->
@@ -331,18 +364,87 @@ Theorem triple_fun_generic_dijkstra
   l_is_nil_spec       l_is_nil ->
   l_head_spec         l_head ->
   l_tail_spec         l_tail ->
-  exists c0 c2, forall n,
+  exists c0 cn cm, forall (g : wgraph nat) vg src D pred n m C t,
   is_set_size (V g) n ->
+  is_set_size (uncurry (E g)) m ->
+  is_max_label g C ->
+  heap_time_bound n C t ->
   triple_fun
     (generic_dijkstra
-      get_size get_neighbours get_max_label mkheap h_insert h_empty
+      get_size get_max_label get_neighbours mkheap h_insert h_empty
       h_extract_min h_decrease_key h_free l_is_nil l_head l_tail)
-    (fun v => <[v = Lab l]>)
+    (fun v => $1 <*> <[v = vg]>)
     (fun v => <[triple_fun v
-      (fun v => <[v = Int (Z.of_nat src)]> <*> is_weighted_graph g (Lab l) <*>
-        <[V g src]> <*> <[Dijkstra_initial D pred src]> <*> sa_credits (c0 + c2*n*n))
-      (fun v => <exists> lD lpred c, <[v = RecV [Lab lD; Lab lpred]]> <*>
-        is_weighted_graph g (Lab l) <*> is_nat_function D lD <*>
-        is_nat_function pred lpred <*> <[Dijkstra_final D pred src g]> <*> sa_credits c)]>).
-Proof.
+      (fun v => $ (c0 + cm*m + cn*n*t) <*> <[v = Int (Z.of_nat src)]> <*>
+        is_weighted_graph g vg <*> <[V g src]> <*> <[Dijkstra_initial D pred src]>)
+      (fun v => (<exists> c, $c) <*> <exists> lD lpred, <[v = RecV [Lab lD; Lab lpred]]> <*>
+        is_weighted_graph g vg <*> is_nat_function D lD <*>
+        is_nat_function pred lpred <*> <[Dijkstra_final D pred src g]>)]>).
+Proof using.
+(*unfold is_closed_value.*)
+  intros Hclosed_get_size Hclosed_get_max_label Hclosed_get_neighbours Hclosed_mkheap
+    Hclosed_h_insert Hclosed_h_empty Hclosed_h_extract_min Hclosed_h_decrease_key
+    Hclosed_h_free Hclosed_l_is_nil Hclosed_l_head Hclosed_l_tail.
+  unfold get_size_spec, get_neighbours_spec, get_max_label_spec, mkheap_spec, h_insert_spec, h_empty_spec,
+    h_extract_min_spec, h_decrease_key_spec, h_free_spec, l_is_nil_spec, l_head_spec, l_tail_spec.
+  intros. eexists ?[c0], ?[cn], ?[cm]. intros. unfold triple_fun, generic_dijkstra, StringLam. simpl. intros.
+  repeat (rewrite map_v_shift_closed; [|repeat apply map_v_closed_value; assumption]).
+  app_lambda. triple_pull_pure. subst. solve_simple_value; [|rewrite_empty_spec; rewrite pure_spec; auto].
+  split_all; auto. intros. cbn. triple_pull_pure. solve_simple_value.
+  rewrite_empty_spec. rewrite pure_spec. split_all; auto. intros.
+  instantiate (c0 := S ?[cc0]). instantiate (cc0 := ?[c0]).
+  triple_pull_1_credit. app_lambda. simpl. subst. solve_simple_value.
+  split_all; auto. intros. cbn. triple_reorder_pure. repeat triple_pull_pure. subst.
+  rewrite bind_v_shift, bind_v_id.
+  instantiate (c0 := S ?[cc0]). instantiate (cc0 := ?[c0]).
+  fold (inc_set string).
+  repeat rewrite bind_v_liftS_shift_swap. repeat rewrite bind_v_shift. repeat rewrite bind_v_id. simpl.
+  triple_pull_1_credit. app_lambda.
+  2:{
+    instantiate (c0 := S ?[cc0]). instantiate (cc0 := ?[c0]). triple_pull_1_credit.
+    eapply triple_weaken, triple_frame, triple_fun_app.
+    { apply implies_spec. intros. swap_star_ctx. normalize_star. swap_star_ctx. eassumption. }
+    { prove_implies_refl. }
+    { apply H. admit. }
+    { solve_simple_value. swap_star. solve_star. eassumption. }
+  }
+  solve_simple_value. split_all; auto. intros. cbn.
+  fold (inc_set (inc_set string)).
+  fold (inc_set string).
+  repeat rewrite bind_v_liftS_shift_swap. repeat rewrite bind_v_shift. repeat rewrite bind_v_id. simpl.
+  instantiate (c0 := S ?[cc0]). instantiate (cc0 := ?[c0]).
+  triple_pull_1_credit. app_lambda.
+  2:{
+    instantiate (c0 := S ?[cc0]). instantiate (cc0 := ?[c0]). triple_pull_1_credit.
+    eapply triple_weaken, triple_frame, triple_fun_app.
+    { apply implies_spec. intros.
+      match goal with
+      | [H : _ ?c ?m |- _ ?c ?m] => eapply star_implies_mono in H
+      end.
+      { apply star_assoc_l. eassumption. }
+      { prove_implies_refl. }
+      { apply implies_spec. intros. swap_star_ctx. apply star_assoc_r.
+        match goal with
+        | [H : _ ?c ?m |- _ ?c ?m] => eapply star_implies_mono in H
+        end.
+        { eassumption. }
+        { apply implies_spec. intros.
+          match goal with
+          | [H : _ ?c ?m |- _ ?c ?m] => apply star_exists_l in H
+          end.
+          swap_star. eassumption. }
+        { prove_implies_refl. } } }
+    { prove_implies_refl. }
+    { apply H0. admit. }
+    { solve_simple_value. swap_star. swap_star_ctx. solve_star. eassumption. }
+  }
+  solve_simple_value. split_all; auto. intros. cbn.
+  fold (inc_set (inc_set (inc_set string))).
+  fold (inc_set (inc_set string)).
+  fold (inc_set string).
+  repeat rewrite bind_v_liftS_shift_swap. repeat rewrite bind_v_shift. repeat rewrite bind_v_id. simpl.
+  (*TODO:
+  triple_pull_exists.
+  triple_reorder_pure.
+  triple_pull_pure.*)
 Admitted.
