src_arrays/SA_Tactics.v
@@ -1,0 +1,587 @@
+Require Import src_arrays.LambdaRef.
+Require Import src_arrays.LambdaAssertions_credits_perm.
+Require Import src_arrays.LambdaTotalTriple_credits_perm.
+Require Import src_arrays.LamRefLogicFactsTotal_credits_perm.
+Require Import List.
+Import ListNotations.
+
+(* state assertion and triple manipulation tactics *)
+
+Ltac extract_exists P H :=
+  match P with
+  | <exists> x, _ => idtac
+  | (<exists> x, _) <*> ?Q' => apply star_exists_l' in H
+  | ?Q <*> (<exists> x, _) => apply star_comm in H; apply star_exists_l' in H
+  | ?Q <*> ?Q' => eapply star_implies_mono in H; [clear H; apply implies_spec; intro H; extract_exists Q H|apply implies_refl]; apply star_exists_l' in H
+  | ?Q <*> ?Q' => apply star_comm in H; eapply star_implies_mono in H; [clear H; apply implies_spec; intro H; extract_exists Q H|apply implies_refl]; extract_exists Q' H; apply star_exists_l' in H
+  end.
+
+Ltac extract_exists_in H :=
+  match type of H with
+  | ?P ?c ?m => extract_exists P H
+  end.
+
+Ltac extract_pure P H :=
+  multimatch P with
+  | <[_]> => idtac
+  | <[_]> <*> ?Q' => idtac
+  | ?Q <*> <[_]> => apply star_comm in H
+  | ?Q <*> ?Q' => eapply star_implies_mono in H; [|clear H; apply implies_spec; intro H; extract_pure Q H|apply implies_refl]; apply star_assoc_l in H
+  | ?Q <*> ?Q' => apply star_comm in H; eapply star_implies_mono in H; [|clear H; apply implies_spec; intro H; extract_pure Q H|apply implies_refl]; apply star_assoc_l in H
+  end.
+
+Ltac extract_pure_in H :=
+  match type of H with
+  | ?P ?c ?m => extract_pure P H
+  end.
+Ltac id' H :=
+  match ltac:(H) with
+  | ?X => exact X
+  end.
+
+Ltac reorder_pure P :=
+  match P with
+  | ?Q <*> ?Q' =>
+    match ltac:(eval simpl in (ltac:(reorder_pure Q) <*> ltac:(reorder_pure Q'))) with
+    | <[?P']> <*> ?Q1' => exact (<[P']> <*> ltac:(reorder_pure Q1'))
+    | (<[?P']> <*> ?Q1) <*> ?Q1' => exact (<[P']> <*> ltac:(reorder_pure (Q1 <*> Q1')))
+    | ?Q1 <*> <[?P']> => exact (<[P']> <*> ltac:(reorder_pure Q1))
+    | ?Q1 <*> (<[?P']> <*> ?Q1') => exact (<[P']> <*> ltac:(reorder_pure (Q1' <*> Q1)))
+    end
+  | _ => exact P
+  end.
+
+Ltac prove_implies_reorder_pure :=
+  match goal with
+  | [|- ?Q <*> ?Q' ->> _] =>
+    eapply implies_trans;
+    [apply star_implies_mono; prove_implies_reorder_pure|];
+    match goal with
+    | [|- <[?P]> <*> ?Q1' ->> _ ] =>
+      apply star_implies_mono; [apply implies_refl|];
+      prove_implies_reorder_pure
+    | [|- (<[?P]> <*> ?Q1) <*> ?Q1' ->> _ ] =>
+      eapply implies_trans; [apply star_assoc_r|];
+      apply star_implies_mono; [apply implies_refl|];
+      prove_implies_reorder_pure
+    | [|- ?Q1 <*> <[?P]> ->> _ ] =>
+      eapply implies_trans; [apply star_comm|];
+      apply star_implies_mono; [apply implies_refl|];
+      prove_implies_reorder_pure
+    | [|- ?Q1 <*> (<[?P]> <*> ?Q1') ->> _ ] =>
+      eapply implies_trans; [apply star_comm|];
+      eapply implies_trans; [apply star_assoc_r|];
+      apply star_implies_mono; [apply implies_refl|];
+      prove_implies_reorder_pure
+    end
+  | [|- ?P ->> _] => apply implies_refl
+  end.
+(*
+Ltac prove_implies_reorder_pure_bwd :=
+  match goal with
+  | [|- _ ->> ?Q <*> ?Q'] =>
+    eapply implies_trans;
+    [|apply star_implies_mono; prove_implies_reorder_pure_bwd];
+    match goal with
+    | [|- _ ->> <[?P]> <*> ?Q1' ] =>
+      apply star_implies_mono; [apply implies_refl|];
+      prove_implies_reorder_pure_bwd
+    | [|- _ ->> (<[?P]> <*> ?Q1) <*> ?Q1' ] =>
+      eapply implies_trans; [|apply star_assoc_r];
+      apply star_implies_mono; [apply implies_refl|];
+      prove_implies_reorder_pure_bwd
+    | [|- _ ->> ?Q1 <*> <[?P]> ] =>
+      eapply implies_trans; [|apply star_comm];
+      apply star_implies_mono; [apply implies_refl|];
+      prove_implies_reorder_pure_bwd
+    | [|- _ ->> ?Q1 <*> (<[?P]> <*> ?Q1') ] =>
+      eapply implies_trans; [|apply star_comm];
+      eapply implies_trans; [|apply star_assoc_r];
+      apply star_implies_mono; [apply implies_refl|];
+      prove_implies_reorder_pure_bwd
+    end
+  | [|- _ ->> ?P] => apply implies_refl
+  end.
+*)
+Ltac triple_reorder_pure :=
+  match goal with
+  | [|- triple ?e ?P' ?Q'] =>
+    apply triple_weaken with (P := ltac:(reorder_pure P')) (Q := Q');
+      [prove_implies_reorder_pure|intros; apply implies_refl|]
+  end.
+
+Ltac triple_pull_pure :=
+  match goal with
+  | [|- triple ?e <[?P]> ?Q] =>
+    apply -> triple_pure; intro
+  | [|- triple ?e (<[?P]> <*> ?Q) ?Q'] =>
+    apply -> triple_pure_star; intro
+  end.
+
+Ltac triple_pull_exists :=
+  match goal with
+  | [|- triple ?e (<exists> _, _) ?Q] =>
+    apply -> triple_exists; intro
+  | [|- triple ?e (?Q <*> <exists> _, _) ?Q'] =>
+    apply -> triple_exists_star; intro
+  end.
+
+Ltac reorder_credits P :=
+  match P with
+  | ?Q <*> ?Q' =>
+    match ltac:(eval simpl in (ltac:(reorder_credits Q) <*> ltac:(reorder_credits Q'))) with
+    | sa_credits ?n <*> ?Q1' => exact (sa_credits n <*> ltac:(reorder_credits Q1'))
+    | (sa_credits ?n <*> ?Q1) <*> ?Q1' => exact (sa_credits n <*> ltac:(reorder_credits (Q1 <*> Q1')))
+    | ?Q1 <*> sa_credits ?n => exact (sa_credits n <*> ltac:(reorder_credits Q1))
+    | ?Q1 <*> (sa_credits ?n <*> ?Q1') => exact (sa_credits n <*> ltac:(reorder_credits (Q1' <*> Q1)))
+    end
+  | _ => exact P
+  end.
+
+(*Check ltac:(reorder_credits (<[]> <*> (<[1=1]> <*> <[2=2]> <*> (sa_credits 2 <*> <[3=3]> <*> sa_credits 4) <*> sa_credits 5) : StateAssertion string)).*)
+
+Ltac prove_implies_reorder_credits :=
+  match goal with
+  | [|- ?Q <*> ?Q' ->> _] =>
+    eapply implies_trans;
+    [apply star_implies_mono; prove_implies_reorder_credits|];
+    match goal with
+    | [|- sa_credits _ <*> ?Q1' ->> _ ] =>
+      apply star_implies_mono; [apply implies_refl|];
+      prove_implies_reorder_credits
+    | [|- (sa_credits _ <*> ?Q1) <*> ?Q1' ->> _ ] =>
+      eapply implies_trans; [apply star_assoc_r|];
+      apply star_implies_mono; [apply implies_refl|];
+      prove_implies_reorder_credits
+    | [|- ?Q1 <*> sa_credits _ ->> _ ] =>
+      eapply implies_trans; [apply star_comm|];
+      apply star_implies_mono; [apply implies_refl|];
+      prove_implies_reorder_credits
+    | [|- ?Q1 <*> (sa_credits _ <*> ?Q1') ->> _ ] =>
+      eapply implies_trans; [apply star_comm|];
+      eapply implies_trans; [apply star_assoc_r|];
+      apply star_implies_mono; [apply implies_refl|];
+      prove_implies_reorder_credits
+    end
+  | [|- ?P ->> _] => apply implies_refl
+  end.
+
+Ltac triple_reorder_credits :=
+  match goal with
+  | [|- triple ?e ?P' ?Q'] =>
+    apply triple_weaken with (P := ltac:(reorder_credits P')) (Q := Q');
+      [prove_implies_reorder_credits|intros; apply implies_refl|]
+  end.
+(*
+Ltac prove_implies_pull_credits n :=
+  match goal with
+  | [|- ?Q <*> ?Q' ->> _] =>
+    eapply implies_trans;
+    [apply star_implies_mono; [prove_implies_pull_credits n|apply implies_refl]|];
+    match goal with
+    | [|- sa_credits _ <*> ?Q1' ->> _ ] => idtac
+    | [|- (sa_credits _ <*> ?Q1) <*> ?Q1' ->> _ ] =>
+      eapply implies_trans; [apply star_assoc_r|]
+    end
+  | [|- ?Q <*> ?Q' ->> _] =>
+    eapply implies_trans;
+    [apply star_implies_mono; [apply implies_refl|prove_implies_pull_credits n]|];
+    match goal with
+    | [|- ?Q1 <*> sa_credits _ ->> _ ] =>
+      eapply implies_trans; [apply star_comm|]
+    | [|- ?Q1 <*> (sa_credits _ <*> ?Q1') ->> _ ] =>
+      eapply implies_trans; [apply star_comm|];
+      eapply implies_trans; [apply star_assoc_r|]
+    end
+  | [|- sa_credits _ <*> ?Q ->> _ ] =>
+    eapply star_implies_mono;
+    [eapply credits_star_r with (c1 := n); reflexivity|apply implies_refl]
+  | [|- sa_credits _ ->> _] => eapply credits_star_r with (c1 := n); reflexivity
+  | [|- ?P ->> _] => apply implies_refl
+  end.
+Ltac triple_pull_credits n :=
+  match goal with
+  | [|- triple ?e ?P' ?Q'] =>
+    eapply triple_weaken with (Q := Q');
+      [prove_implies_reorder_credits n|intros; apply implies_refl|]
+  end.
+*)
+
+Ltac triple_pull_credits n :=
+  match goal with
+  | [|- triple ?e (sa_credits _) ?Q' ] =>
+    eapply triple_weaken with (Q := Q');
+    [eapply credits_star_r with (c1 := n); reflexivity
+    |intros; apply implies_refl
+    |]
+  | [|- triple ?e (sa_credits _ <*> ?P') ?Q' ] =>
+    eapply triple_weaken with (Q := Q');
+    [eapply star_implies_mono;
+      [eapply credits_star_r with (c1 := n); reflexivity|apply implies_refl]
+    |intros; apply implies_refl
+    |]
+  end.
+
+Ltac triple_pull_1_credit :=
+  triple_reorder_credits; triple_pull_credits 1; triple_reorder_credits.
+
+Ltac reorder X P :=
+  match P with
+  | ?Q <*> ?Q' =>
+    match ltac:(eval simpl in (ltac:(reorder X Q) <*> ltac:(reorder X Q'))) with
+    | X <*> ?Q1' => exact (X <*> ltac:(reorder X Q1'))
+    | (X <*> ?Q1) <*> ?Q1' => exact (X <*> ltac:(reorder X (Q1 <*> Q1')))
+    | ?Q1 <*> X => exact (X <*> ltac:(reorder X Q1))
+    | ?Q1 <*> (X <*> ?Q1') => exact (X <*> ltac:(reorder X (Q1' <*> Q1)))
+    end
+  | _ => exact P
+  end.
+(*Check (fun x (y : Expr (_ string)) => ltac:(reorder (<(x :== -\ y)>) (<[]> <*> <[1=1]> <*> (<[2=2]> <*> (<[3=3]> <*> <[]> <*> <[4=4]> <*> (<[5=5]> <*> <(x :== -\ y)>) <*> <[6=6]>))))).*)
+Ltac prove_implies_reorder X :=
+  match goal with
+  | [|- ?Q <*> ?Q' ->> _] =>
+    eapply implies_trans;
+    [apply star_implies_mono; prove_implies_reorder X|];
+    match goal with
+    | [|- X <*> ?Q1' ->> _ ] =>
+      apply star_implies_mono; [apply implies_refl|];
+      prove_implies_reorder X
+    | [|- (X <*> ?Q1) <*> ?Q1' ->> _ ] =>
+      eapply implies_trans; [apply star_assoc_r|];
+      apply star_implies_mono; [apply implies_refl|];
+      prove_implies_reorder X
+    | [|- ?Q1 <*> X ->> _ ] =>
+      eapply implies_trans; [apply star_comm|];
+      apply star_implies_mono; [apply implies_refl|];
+      prove_implies_reorder X
+    | [|- ?Q1 <*> (X <*> ?Q1') ->> _ ] =>
+      eapply implies_trans; [apply star_comm|];
+      eapply implies_trans; [apply star_assoc_r|];
+      apply star_implies_mono; [apply implies_refl|];
+      prove_implies_reorder X
+    end
+  | [|- ?P ->> _] => apply implies_refl
+  end.
+
+Ltac prove_implies_reorder_bwd X :=
+  match goal with
+  | [|- _ ->> ?Q <*> ?Q'] =>
+    eapply implies_trans;
+    [|apply star_implies_mono; prove_implies_reorder_bwd X];
+    match goal with
+    | [|- _ ->> X <*> ?Q1' ] =>
+      apply star_implies_mono; [apply implies_refl|];
+      prove_implies_reorder_bwd X
+    | [|- _ ->> (X <*> ?Q1) <*> ?Q1' ] =>
+      eapply implies_trans; [|apply star_assoc_l];
+      apply star_implies_mono; [apply implies_refl|];
+      prove_implies_reorder_bwd X
+    | [|- _ ->> ?Q1 <*> X ] =>
+      eapply implies_trans; [|apply star_comm];
+      apply star_implies_mono; [apply implies_refl|];
+      prove_implies_reorder_bwd X
+    | [|- _ ->> ?Q1 <*> (X <*> ?Q1') ] =>
+      eapply implies_trans; [|apply star_comm];
+      eapply implies_trans; [|apply star_assoc_l];
+      apply star_implies_mono; [apply implies_refl|];
+      prove_implies_reorder_bwd X
+    end
+  | [|- ?P ->> _] => apply implies_refl
+  end.
+
+Ltac triple_reorder X :=
+  match goal with
+  | [|- triple ?e ?P' ?Q'] =>
+    eapply triple_weaken with (P := ltac:(reorder X P')) (Q := Q');
+      [prove_implies_reorder X|intros; apply implies_refl|]
+  end.
+
+Ltac prove_implies_refl :=
+  intros; simpl; apply implies_refl.
+
+Ltac rewrite_empty_spec :=
+  match goal with
+  | [H : <[]> ?c ?m |- _] => apply empty_spec in H as (->&->)
+  end.
+
+Ltac unify_not_evar X Y :=
+  not_evar Y; unify X Y.
+
+Ltac remove X P :=
+  lazymatch ltac:(type of X) with
+  | StateAssertion ?V =>
+    match P with
+    | ?Y => unify_not_evar X Y; exact (sa_empty : StateAssertion V)
+    | ?Q <*> ?Q' =>
+      match ltac:(eval simpl in (ltac:(remove X Q))) with
+      | <[]> => exact Q'
+      | ?Q1 => exact (Q1 <*> Q')
+      end
+    | ?Q <*> ?Q' =>
+      match ltac:(eval simpl in (ltac:(remove X Q'))) with
+      | <[]> => exact Q
+      | ?Q1' => exact (Q <*> Q1')
+      end
+    end
+  end.
+
+Ltac prove_implies_reorder1 X :=
+  match goal with
+  | [|- ?Y ->> _] => unify_not_evar X Y; apply implies_refl
+  | [|- ?Q <*> ?Q' ->> _] =>
+    eapply implies_trans;
+    [apply star_implies_mono; [prove_implies_reorder1 X|apply implies_refl]|];
+    lazymatch goal with
+    | [|- (?Y <*> ?Q1) <*> ?Q1' ->> _ ] => unify_not_evar X Y; apply star_assoc_r
+    | [|- ?Y <*> ?Q1' ->> _ ] => unify_not_evar X Y; apply implies_refl
+    end
+  | [|- ?Q <*> ?Q' ->> _] =>
+    eapply implies_trans;
+    [apply star_implies_mono; [apply implies_refl|prove_implies_reorder1 X]|];
+    lazymatch goal with
+    | [|- ?Q1 <*> (?Y <*> ?Q1') ->> _ ] =>
+      unify_not_evar X Y;
+      eapply implies_trans;
+      [apply star_assoc_l|];
+      eapply implies_trans;
+      [apply star_implies_mono; [apply star_comm|apply implies_refl]|];
+      apply star_assoc_r
+    | [|- ?Q1 <*> ?Y ->> _ ] => unify_not_evar X Y; apply star_comm
+    end
+  | [|- ?P ->> ?Q] => unify_not_evar Q P; apply implies_refl
+  end.
+
+Ltac prove_implies_reorder1_bwd X :=
+  match goal with
+  | [|- _ ->> ?Y] => unify_not_evar X Y; apply implies_refl
+  | [|- _ ->> ?Q <*> ?Q'] =>
+    eapply implies_trans;
+    [|apply star_implies_mono; [prove_implies_reorder1_bwd X|apply implies_refl]];
+    lazymatch goal with
+    | [|- _ ->> (?Y <*> ?Q1) <*> ?Q1' ] => unify_not_evar X Y; apply star_assoc_l
+    | [|- _ ->> ?Y <*> ?Q1' ] => unify_not_evar X Y; apply implies_refl
+    end
+  | [|- _ ->> ?Q <*> ?Q'] =>
+    eapply implies_trans;
+    [|apply star_implies_mono; [apply implies_refl|prove_implies_reorder1_bwd X]];
+    lazymatch goal with
+    | [|- _ ->> ?Q1 <*> (?Y <*> ?Q1') ] =>
+      unify_not_evar X Y;
+      eapply implies_trans;
+      [|apply star_assoc_r];
+      eapply implies_trans;
+      [|apply star_implies_mono; [apply star_comm|apply implies_refl]];
+      apply star_assoc_l
+    | [|- _ ->> ?Q1 <*> ?Y ] => unify_not_evar X Y; apply star_comm
+    end
+  | [|- ?P ->> ?Q] => unify_not_evar P Q; apply implies_refl
+  end.
+
+Ltac triple_reorder1 X :=
+  match goal with
+  | [|- triple ?e ?P' ?Q'] =>
+    apply triple_weaken with (P := X <*> ltac:(remove X P')) (Q := Q');
+      [prove_implies_reorder1 X|prove_implies_refl|]
+  end.
+
+Ltac clear_empty P :=
+  lazymatch P with
+  | ?Q <*> ?Q' => (*idtac Q Q';*)
+    match ltac:(eval simpl in (ltac:(clear_empty Q) <*> ltac:(clear_empty Q'))) with
+    | <[]> <*> ?Q1' => (*idtac 1 Q1';*) exact Q1'
+    | ?Q1 <*> <[]> => (*idtac 2 Q1;*) exact Q1
+    | ?Q1 => (*idtac 3 Q1;*) exact Q1
+    end
+  | <exists> t : ?T, @?Q t => (*idtac t T Q;*)
+    let Q' := ltac:(eval simpl in ltac:(clear_empty Q)) in
+    (*idtac T Q'; idtac ">";*) exact (<exists> t : T, Q' t) (*; idtac "OK") || idtac "!")*)
+  | fun t : ?T => @?Q t => (*idtac t T Q;*)
+    let u := fresh t in(*exact (fun x : T => ltac:(eval simpl in ltac:(clear_empty Q)))*)
+    let Q' := ltac:(eval simpl in (fun u =>ltac:(clear_empty ltac:(eval simpl in (Q u))))) in
+    (*idtac t T Q'; idtac ">!";*) exact Q' (*; idtac "OK!") || idtac "!!")*)
+  | _ => exact P (*; idtac "<>"*)
+  end.
+
+(*Goal True.
+match constr:(fun x => x + 1) with
+| fun t => @?y t => let a := fresh t in let b := constr:(fun a => y a) in idtac a b y
+end.
+Abort.
+Check (ltac:(clear_empty ltac:(eval simpl in (fun (x:Label) (y : Expr (inc_set string)) =>  (<[]> <*> <[1=1]> <*> (<[2=2]> <*> <exists> n m : nat, (<[n=m]> <*> <[]> <*> <[4=4]> <*> (<[5=5]> <*> <(x :== -\y)>) <*> <[]> <*> <[6=6]>)):StateAssertion string))))).
+Goal True. match constr:(fun x xx : nat => ((fun t => t + xx) x + 1) * 3) with
+| fun z v => @?y z v * 3 => idtac "y =" y; pose (fun z : nat => ltac:(
+  match ltac:(eval simpl in (fun v : nat => y z v)) with
+  | fun r => @?a r => idtac "r =" r "; a =" a; let aa := (ltac:(eval simpl in (a))) in exact (aa 8)
+  end) * 5)
+end.*)
+
+Ltac prove_implies_clear_empty :=
+  lazymatch goal with
+  | [|- ?Q <*> ?Q' ->> _ ] =>
+    eapply implies_trans;
+    [apply star_implies_mono; prove_implies_clear_empty|];
+    lazymatch goal with
+    | [|- <[]> <*> ?Q1' ->> _] => apply empty_star_l_cancel
+    | [|- ?Q1 <*> <[]> ->> _] => apply empty_star_r_cancel
+    | [|- ?Q1 ->> _] => apply implies_refl
+    end
+  | [|- (<exists> x, @?P' x) ->> _] =>
+    apply exists_implies with (P := P'); prove_implies_clear_empty
+  | [|- forall x, ?Q ->> _] =>
+    intros; prove_implies_clear_empty
+  | [|- ?P ->> _] => apply implies_refl
+  end.
+
+Ltac prove_implies_clear_empty_bwd :=
+  lazymatch goal with
+  | [|- _ ->> ?Q <*> ?Q' ] =>
+    eapply implies_trans;
+    [|apply star_implies_mono; prove_implies_clear_empty_bwd];
+    lazymatch goal with
+    | [|- _ ->> <[]> <*> ?Q1'] => apply empty_star_l_intro
+    | [|- _ ->> ?Q1 <*> <[]>] => apply empty_star_r_intro
+    | [|- _ ->> ?Q1] => apply implies_refl
+    end
+  | [|- _ ->> (<exists> x, @?Q' x)] =>
+    apply exists_implies with (Q := Q'); prove_implies_clear_empty_bwd
+  | [|- forall x, ?Q ->> _] =>
+    intros; prove_implies_clear_empty_bwd
+  | [|- _ ->> ?P] => apply implies_refl
+  end.
+
+Ltac triple_clear_empty :=
+  match goal with
+  | [|- triple ?e ?P' ?Q'] =>
+    apply triple_weaken with (P := ltac:(clear_empty P')) (Q := Q');
+      [prove_implies_clear_empty|prove_implies_refl|]
+  end.
+
+Ltac triple_clear_empty_r :=
+  match goal with
+  | [|- triple ?e ?P' ?Q'] =>
+    apply triple_weaken with (P := P') (Q := ltac:(clear_empty Q'));
+      [prove_implies_refl|prove_implies_clear_empty_bwd|]
+  end.
+(*Check (fun x (y : Expr (_ string)) => ltac:(clear_empty ltac:(eval simpl in ltac:(remove (<(x :== -\y)>) (<[]> <*> <[1=1]> <*> (<[2=2]> <*> (<[3=3]> <*> <[]> <*> <[4=4]> <*> (<[5=5]> <*> <(x :== -\ y)>) <*> <[]> <*> <[6=6]>))))))).*)
+(*
+Goal True.
+eassert (option (Value string)). shelve.
+eassert (H = _). shelve.
+lazymatch goal with
+| [_ : H = ?yy |- _] =>
+  epose (fun x (y : Expr (_ string)) => ltac:(clear_empty ltac:(eval simpl in ltac:(remove (<(x :?= Some (-\ y))> : StateAssertion string) (<[]> <*> <[1=1]> <*> (<[2=2]> <*> (<[3=3]> <*> <[]> <*> <[4=4]> <*> (<[5=5]> <*> <(x :== -\ y)>) <*> <[]> <*> <[6=6]>)))))))
+end.
+lazymatch goal with
+| [_ : H = ?yy |- _] =>
+  epose (fun x (y : Expr (_ string)) => ltac:(clear_empty ltac:(eval simpl in ltac:(remove (<(x :?= yy)> : StateAssertion string) (<[]> <*> <[1=1]> <*> (<[2=2]> <*> (<[3=3]> <*> <[]> <*> <[4=4]> <*> (<[5=5]> <*> <(x :== @U_val string)>) <*> <[]> <*> <[6=6]>)))))))
+end.
+Abort.
+
+Ltac tmp P :=
+  lazymatch P with
+  | ?Q <*> ?Q' => (*idtac Q Q';*)
+    tmp Q; tmp Q'
+  | <exists> t : ?T, @?Q t => (*idtac t T Q;*)
+    tmp Q
+  | fun t : ?T => @?Q t => (*idtac t T Q;*)
+    let u := fresh t in(*exact (fun x : T => ltac:(eval simpl in ltac:(clear_empty Q)))*)
+    tmp (Q u)
+  | ?X => (is_evar X; idtac "is_evar -" X) || idtac "!" X
+  end.
+*)
+
+Ltac get_leftmost P :=
+  lazymatch P with
+  | ?Q <*> ?Q' => exact ltac:(get_leftmost Q)
+  | _ => exact P
+  end.
+
+Ltac reorder_leftmost P :=
+  let l := (ltac:(eval simpl in ltac:(get_leftmost P))) in
+  exact (l <*> ltac:(remove l P)).
+(*Check (fun x (y : Expr (_ string)) => ltac:(reorder_leftmost (((<[1=1]> <*> <[8=8]>) <*> <[7=7]>) <*> (<[2=2]> <*> (<[3=3]> <*> <[]> <*> <[4=4]> <*> (<[5=5]> <*> <(x :== -\ y)>) <*> <[]> <*> <[6=6]>))))).*)
+Ltac prove_implies1 :=
+  lazymatch goal with
+  | [|- ?P ->> ?QQ] =>
+    (unify P QQ; apply implies_refl) ||
+    (let l := (ltac:(eval simpl in ltac:(get_leftmost P))) in
+     let P' := (ltac:(eval simpl in ltac:(remove l P))) in
+     let Q' := (ltac:(eval simpl in ltac:(remove l QQ))) in
+     apply implies_trans with (Q := l <*> P');
+     [prove_implies_reorder1 l|];
+     apply implies_trans with (Q := l <*> Q');
+     [|prove_implies_reorder1_bwd l];
+     apply star_implies_mono;
+     [apply implies_refl|])
+  end.
+
+Ltac prove_implies1_rev :=
+  lazymatch goal with
+  | [|- ?P ->> ?QQ] =>
+    (unify P QQ; apply implies_refl) ||
+    (let l := (ltac:(eval simpl in ltac:(get_leftmost QQ))) in
+     let P' := (ltac:(eval simpl in ltac:(remove l P))) in
+     let Q' := (ltac:(eval simpl in ltac:(remove l QQ))) in
+     apply implies_trans with (Q := l <*> Q');
+     [|prove_implies_reorder1_bwd l];
+     apply implies_trans with (Q := l <*> P');
+     [prove_implies_reorder1 l|];
+     apply star_implies_mono;
+     [apply implies_refl|])
+  end.
+
+Ltac prove_implies :=
+  repeat prove_implies1.
+Ltac prove_implies_rev :=
+  repeat prove_implies1_rev.
+
+Ltac fold_implies :=
+  lazymatch goal with
+  | [|- forall c m, ?P c m -> ?Q c m] => fold (P ->> Q)
+  end.
+
+Ltac revert_implies :=
+  lazymatch goal with
+  | [H : ?P ?c ?m |- ?Q ?c ?m] => revert c m H; fold_implies
+  end.
+
+Ltac triple_value_revert :=
+  match goal with
+  | [v : Value _ |- triple (Val ?v') _ _] => unify v v'; generalize dependent v
+  | [|- triple (Val ?v') _ _] => remember v' as t; generalize dependent t
+  end.
+
+Ltac eta_expand_pre_triple_value :=
+  triple_value_revert;
+  lazymatch goal with
+  | [|- forall v : ?T, triple (Val v) (@?P v) ?Q] =>
+    change (forall v : T, triple v (P v) Q)
+  | [|- forall (v : ?T) (x : ?H), triple (Val v) (@?P v) ?Q] =>
+    change (forall (v : T) (x : H), triple v (P v) Q)
+  end;
+  intros.
+
+Ltac solve_simple_value :=
+  apply triple_value_implies; apply implies_spec; intros; solve_star;
+  try eassumption.
+
+Ltac solve_value_unify :=
+  match goal with
+  | [|- triple (Val ?v) ?P ?Q] =>
+    unify P (Q v); apply triple_value_implies; apply implies_refl
+  end.
+
+Ltac app_lambda :=
+  lazymatch goal with
+  | [|- triple (Val (-\ ?e1') <* Val ?v2) (sa_credits 1 <*> ?P) ?Q] => (*idtac e1' v2 P Q;*)
+    eapply triple_app with (P2 := P); [|eta_expand_pre_triple_value; solve_value_unify]
+  | [|- triple (Val (-\ ?e1') <* ?e2) (sa_credits 1 <*> ?P) ?Q] => (*idtac e1' e2 P Q;*)
+    eapply triple_app with (P2 := P)
+  end.
+
+Ltac triple_expand_empty_pre_r :=
+  lazymatch goal with
+  | [|- triple ?e ?P' ?Q'] =>
+    apply triple_weaken with (P := P' <*> <[]>) (Q := Q');
+      [apply empty_star_r_intro|prove_implies_refl|]
+  end.
